fiat2/src/fiat2/Utils.v
@@ -897,6 +897,15 @@ Section WithMap.
     | H: locals_equiv ?G _ _, H': map.get ?G _ = Some _ |- _ =>
         apply H in H' end.
 
+  Lemma In_flat_map2_ext : forall (A B C : Type) (l : list A) (l' : list B) (f g : A -> B -> list C),
+      (forall a b, In a l -> In b l' -> f a b = g a b) -> flat_map2 f l l' = flat_map2 g l l'.
+  Proof.
+    induction l; auto.
+    destruct l'; auto.
+    cbn; intros. rewrite H; auto.
+    f_equal. erewrite IHl; eauto.
+  Qed.
+
   Ltac use_interp_expr__locals_equiv_IH :=
     lazymatch goal with
       IH: context[interp_expr _ _ ?e] |- context[interp_expr _ _ ?e] =>
@@ -927,6 +936,13 @@ Section WithMap.
         apply In_flat_map_ext; intros.
         Forall_fst__Forall_bag_to_list. apply_Forall_In.
         use_interp_expr__locals_equiv_IH; [ | | | eauto | .. ]; eauto with fiat2_hints. }
+    1:{ repeat (use_interp_expr__locals_equiv_IH; [ | | | eauto | .. ]; eauto).
+        apply_type_sound e1; invert_type_of_value.
+        apply_type_sound e2; invert_type_of_value.
+        f_equal.
+        apply In_flat_map2_ext; intros. repeat apply_Forall_In.
+        use_interp_expr__locals_equiv_IH; [ | | | eauto | .. ];
+          try apply tenv_wf_step; try apply locals_wf_step; eauto with fiat2_hints. }
     1:{ use_interp_expr__locals_equiv_IH; [ | | | eauto | .. ]; eauto.
         apply_type_sound e1; invert_type_of_value.
         revert IHe3. use_interp_expr__locals_equiv_IH; [ | | | eauto | .. ]; eauto; intros.
@@ -1124,7 +1140,7 @@ Section WithMap.
     all: try now (repeat destruct_match_hyp; try congruence;
                   try do_injection;
                   repeat (use_synthesize_ty_unique_IH; eauto with fiat2_hints);
-                  try congruence; repeat (try clear_refl; do_injection); subst; eauto; repeat (try clear_refl; do_injection); f_equal; use_synthesize_ty_unique_IH;
+                  try congruence; repeat (try clear_refl; do_injection); subst; eauto; repeat (try clear_refl; do_injection); try (f_equal; use_synthesize_ty_unique_IH);
                   repeat apply tenv_wf_step; eauto with fiat2_hints).
     1:{ do_injection. inversion H; subst; eauto. }
     1:{ repeat destruct_match_hyp; try congruence;
@@ -1501,6 +1517,9 @@ Fixpoint free_immut_in (x : string) (e : expr) : bool :=
   | ETernop _ e1 e2 e3 => free_immut_in x e1 || free_immut_in x e2 || free_immut_in x e3
   | EIf e1 e2 e3 => free_immut_in x e1 || free_immut_in x e2 || free_immut_in x e3
   | ELet e1 y e2 | EFlatmap _ e1 y e2 => free_immut_in x e1 || (negb (String.eqb x y) && free_immut_in x e2)
+  | EFlatmap2 e1 e2 x1 x2 e3 =>
+      free_immut_in x e1 || free_immut_in x e2 ||
+        (negb (String.eqb x x1) && negb (String.eqb x x2) && free_immut_in x e3)
   | EFold e1 e2 y z e3 => free_immut_in x e1 || free_immut_in x e2 || (negb (String.eqb x y) && negb (String.eqb x z) && free_immut_in x e3)
   | EACFold _ e => free_immut_in x e
   | ERecord l => existsb (fun '(_, e) => free_immut_in x e) l
@@ -1548,11 +1567,21 @@ Section WithMap.
         * apply IHe2; intuition.
           rewrite eqb_neq in *. rewrite Properties.map.put_put_diff; auto.
     - inversion H0; subst; econstructor.
-      1,3: apply IHe1; eauto; intuition.
+      1,3: apply IHe1; eauto; intuition idtac.
       1,2: destruct (x =? x0) eqn:Ex;
       [ rewrite eqb_eq in *; subst; rewrite Properties.map.put_put_same in *; auto
       | apply IHe2; intuition idtac;
         rewrite eqb_neq in *; rewrite Properties.map.put_put_diff; auto ].
+    - invert_type_of_clear; econstructor.
+      1: apply IHe1; eauto; intuition idtac.
+      1: apply IHe2; eauto; intuition idtac.
+      destruct (x =? x1) eqn:Ex1;
+      [ rewrite eqb_eq in *; subst; rewrite Properties.map.put_put_same in *; auto
+      | rewrite eqb_neq in *; rewrite Properties.map.put_put_diff with (k1 := x) in *; auto ].
+      destruct (x =? x2) eqn:Ex2;
+        [ rewrite eqb_eq in *; subst; rewrite Properties.map.put_put_same in *; auto
+        | apply IHe3; intuition idtac;
+          rewrite eqb_neq in *; rewrite Properties.map.put_put_diff; auto ].
     - inversion H0; subst; econstructor.
       + apply IHe1; eauto; intuition.
       + apply IHe2; intuition.
@@ -1641,6 +1670,17 @@ Section WithMap.
       rewrite Properties.map.put_put_same; auto.
       1,2: rewrite eqb_neq in *; rewrite Properties.map.put_put_diff; auto;
       erewrite IHe2; intuition.
+    - rewrite <- IHe1; intuition idtac.
+      rewrite <- IHe2; intuition idtac.
+      repeat case_match; auto. f_equal.
+      apply In_flat_map2_ext; intros.
+      destruct (x =? x1) eqn:Ex1;
+        [ rewrite eqb_eq in *; subst; rewrite Properties.map.put_put_same; auto
+        | rewrite eqb_neq in *; rewrite Properties.map.put_put_diff with (k1 := x); intuition idtac ].
+      destruct (x =? x2) eqn:Ex2;
+        [ rewrite eqb_eq in *; subst; rewrite Properties.map.put_put_same; auto
+        | rewrite eqb_neq in *; rewrite Properties.map.put_put_diff with (k1 := x); intuition idtac ].
+      rewrite <- (IHe3 x); auto.
     - rewrite <- IHe1; intuition. case_match; auto. rewrite <- IHe2; auto.
       apply In_fold_right_ext with (P := fun _ => True); auto.
       intros. destruct (x0 =? x) eqn:Ex.
